concurrency/erased_machine.v
@@ -1,0 +1,204 @@
+Require Import compcert.lib.Axioms.
+
+Require Import concurrency.sepcomp. Import SepComp.
+Require Import sepcomp.semantics_lemmas.
+Require Import concurrency.pos.
+Require Import concurrency.scheduler.
+Require Import concurrency.concurrent_machine.
+Require Import concurrency.addressFiniteMap. (*The finite maps*)
+Require Import concurrency.pos.
+Require Import concurrency.lksize.
+Require Import Coq.Program.Program.
+From mathcomp.ssreflect Require Import ssreflect ssrbool ssrnat ssrfun eqtype seq fintype finfun.
+Set Implicit Arguments.
+
+(*NOTE: because of redefinition of [val], these imports must appear 
+  after Ssreflect eqtype.*)
+Require Import compcert.common.AST.     (*for typ*)
+Require Import compcert.common.Values. (*for val*)
+Require Import compcert.common.Globalenvs. 
+Require Import compcert.common.Memory.
+Require Import compcert.lib.Integers.
+Require Import concurrency.threads_lemmas.
+
+Require Import Coq.ZArith.ZArith.
+
+Notation EXIT := 
+  (EF_external "EXIT" (mksignature (AST.Tint::nil) None)). 
+
+Notation CREATE_SIG :=
+  (mksignature (AST.Tint::AST.Tint::nil) (Some AST.Tint) cc_default).
+Notation CREATE := (EF_external "spawn" CREATE_SIG).
+
+Notation READ := 
+  (EF_external "READ" (mksignature (AST.Tint::AST.Tint::AST.Tint::nil)
+                                   (Some AST.Tint) cc_default)).
+Notation WRITE := 
+  (EF_external "WRITE" (mksignature (AST.Tint::AST.Tint::AST.Tint::nil)
+                                    (Some AST.Tint) cc_default)).
+
+Notation MKLOCK := 
+  (EF_external "makelock" (mksignature (AST.Tint::nil)
+                                     (Some AST.Tint) cc_default)).
+Notation FREE_LOCK := 
+  (EF_external "freelock" (mksignature (AST.Tint::nil)
+                                        (Some AST.Tint) cc_default)).
+
+Notation LOCK_SIG := (mksignature (AST.Tint::nil) (Some AST.Tint) cc_default).
+Notation LOCK := (EF_external "acquire" LOCK_SIG).
+Notation UNLOCK_SIG := (mksignature (AST.Tint::nil) (Some AST.Tint) cc_default).
+Notation UNLOCK := (EF_external "release" UNLOCK_SIG).
+
+Require Import concurrency.permissions.
+Require Import concurrency.threadPool.
+
+Module LocksAndResources.
+  Definition res : Type := unit.
+  Definition lock_info : Type := unit.
+End LocksAndResources.
+
+Module ThreadPool (SEM:Semantics)  <: ThreadPoolSig
+    with Module TID:= NatTID with Module SEM:=SEM
+    with Module RES := LocksAndResources.
+    Include (OrdinalPool SEM LocksAndResources).
+End ThreadPool.
+
+
+Module mySchedule := ListScheduler NatTID.
+
+Module ErasedMachineShell (SEM:Semantics)  <: ConcurrentMachineSig
+    with Module ThreadPool.TID:=mySchedule.TID
+    with Module ThreadPool.SEM:= SEM
+    with Module ThreadPool.RES:= LocksAndResources
+    with Module Events.TID := mySchedule.TID.
+
+   Module Events := Events.
+   Module ThreadPool := ThreadPool SEM.
+   Import ThreadPool.
+   Import ThreadPool.SEM ThreadPool.RES.
+   Import event_semantics Events.
+   
+   Notation tid := NatTID.tid.
+
+   (** Memories*)
+   Definition richMem: Type:= mem.
+   Definition dryMem: richMem -> mem:= id.
+   Definition diluteMem: mem -> mem := erasePerm.
+   
+   Notation thread_pool := (ThreadPool.t).
+   Notation perm_map := ThreadPool.RES.res.
+   
+   (** The state respects the memory*)
+   Definition mem_compatible (tp : thread_pool) (m : mem) : Prop := True.
+
+   Definition invariant (tp : thread_pool) := True.
+   
+   (** Steps*)
+   Inductive dry_step genv {tid0 tp m} (cnt: containsThread tp tid0)
+             (Hcompatible: mem_compatible tp m) :
+     thread_pool -> mem -> seq mem_event -> Prop :=
+   | step_dry :
+       forall (tp':thread_pool) c m' (c' : code) ev
+         (Hcode: getThreadC cnt = Krun c)
+         (Hcorestep: ev_step Sem genv c m ev c' m')
+         (Htp': tp' = updThreadC cnt (Krun c')),
+     dry_step genv cnt Hcompatible tp' m' ev.
+
+   Inductive ext_step (genv:G) {tid0 tp m} (*Can we remove genv from here?*)
+             (cnt0:containsThread tp tid0)(Hcompat:mem_compatible tp m):
+     thread_pool -> mem -> sync_event -> Prop :=
+   | step_acquire :
+       forall (tp' : thread_pool) c m' b ofs
+         (Hcode: getThreadC cnt0 = Kblocked c)
+         (Hat_external: at_external Sem c =
+                        Some (LOCK, ef_sig LOCK, Vptr b ofs::nil))
+         (Hload: Mem.load Mint32 m b (Int.intval ofs) = Some (Vint Int.one))
+         (Hstore: Mem.store Mint32 m b (Int.intval ofs) (Vint Int.zero) = Some m')
+         (Htp': tp' = updThreadC cnt0 (Kresume c Vundef)),
+         ext_step genv cnt0 Hcompat tp' m' (acquire (b, Int.intval ofs))
+                  
+   | step_release :
+       forall (tp':thread_pool) c m' b ofs
+         (Hcode: getThreadC cnt0 = Kblocked c)
+         (Hat_external: at_external Sem c =
+                        Some (UNLOCK, ef_sig UNLOCK, Vptr b ofs::nil))
+         (Hstore: Mem.store Mint32 m b (Int.intval ofs) (Vint Int.one) = Some m')
+         (Htp': tp' = updThreadC cnt0 (Kresume c Vundef)),
+         ext_step genv cnt0 Hcompat tp' m' (release (b, Int.intval ofs))
+                  
+   | step_create :
+       forall (tp_upd tp':thread_pool) c b ofs arg
+         (Hcode: getThreadC cnt0 = Kblocked c)
+         (Hat_external: at_external Sem c =
+                        Some (CREATE, ef_sig CREATE, Vptr b ofs::arg::nil))
+         (Htp_upd: tp_upd = updThreadC cnt0 (Kresume c Vundef))
+         (Htp': tp' = addThread tp_upd (Vptr b ofs) arg tt),
+         ext_step genv cnt0 Hcompat tp' m (spawn (b, Int.intval ofs))
+                  
+   | step_mklock :
+       forall  (tp': thread_pool) c m' b ofs
+          (Hcode: getThreadC cnt0 = Kblocked c)
+          (Hat_external: at_external Sem c =
+                         Some (MKLOCK, ef_sig MKLOCK, Vptr b ofs::nil))
+          (Hstore: Mem.store Mint32 m b (Int.intval ofs) (Vint Int.zero) = Some m')
+          (Htp': tp' = updThreadC cnt0 (Kresume c Vundef)),
+         ext_step genv cnt0 Hcompat tp' m' (mklock (b, Int.intval ofs))
+                  
+   | step_freelock :
+       forall (tp' tp'': thread_pool) c b ofs
+         (Hcode: getThreadC cnt0 = Kblocked c)
+         (Hat_external: at_external Sem c =
+                        Some (FREE_LOCK, ef_sig FREE_LOCK, Vptr b ofs::nil))
+         (Htp': tp' = updThreadC cnt0 (Kresume c Vundef)),
+         ext_step genv cnt0 Hcompat  tp' m (freelock (b,Int.intval ofs))
+                  
+   | step_acqfail :
+       forall  c b ofs
+          (Hcode: getThreadC cnt0 = Kblocked c)
+          (Hat_external: at_external Sem c =
+                         Some (LOCK, ef_sig LOCK, Vptr b ofs::nil))
+          (Hload: Mem.load Mint32 m b (Int.intval ofs) = Some (Vint Int.zero)),
+         ext_step genv cnt0 Hcompat tp m (failacq (b, Int.intval ofs)).
+   
+   Definition threadStep (genv : G): forall {tid0 ms m},
+       containsThread ms tid0 -> mem_compatible ms m ->
+       thread_pool -> mem -> seq mem_event -> Prop:=
+     @dry_step genv.
+   
+   Definition syncStep (genv :G) :
+     forall {tid0 ms m},
+       containsThread ms tid0 -> mem_compatible ms m ->
+       thread_pool -> mem -> sync_event -> Prop:=
+     @ext_step genv.
+
+   Inductive threadHalted': forall {tid0 ms},
+       containsThread ms tid0 -> Prop:=
+   | thread_halted':
+       forall tp c tid0
+         (cnt: containsThread tp tid0)
+         (Hcode: getThreadC cnt = Krun c)
+         (Hcant: halted Sem c),
+         threadHalted' cnt.
+   
+   Definition threadHalted: forall {tid0 ms},
+       containsThread ms tid0 -> Prop:= @threadHalted'.
+   
+   Definition one_pos : pos := mkPos NPeano.Nat.lt_0_1.
+   
+   Definition initial_machine c :=
+     ThreadPool.mk
+       one_pos
+       (fun _ =>  Kresume c Vundef)
+       (fun _ => tt)
+       empty_lset.
+
+   Definition init_mach (_ : option unit) (genv:G)
+              (v:val)(args:list val):option thread_pool :=
+     match initial_core Sem genv v args with
+     | Some c =>      
+       Some (initial_machine c)
+     | None => None
+     end.
+     
+End ErasedMachineShell.
+
