concurrency/x86_safe.v
@@ -1,0 +1,73 @@
+Require Import compcert.lib.Axioms.
+
+Require Import concurrency.sepcomp. Import SepComp.
+Require Import sepcomp.semantics_lemmas.
+
+Require Import concurrency.pos.
+
+From mathcomp.ssreflect Require Import ssreflect ssrbool ssrnat ssrfun eqtype seq fintype finfun.
+Set Implicit Arguments.
+
+(*NOTE: because of redefinition of [val], these imports must appear 
+  after Ssreflect eqtype.*)
+Require Import compcert.common.AST.     (*for typ*)
+Require Import compcert.common.Values. (*for val*)
+Require Import compcert.common.Globalenvs. 
+Require Import compcert.common.Memory.
+Require Import compcert.common.Events.
+Require Import compcert.lib.Integers.
+
+Require Import Coq.ZArith.ZArith.
+
+Require Import concurrency.threads_lemmas.
+Require Import concurrency.permissions.
+Require Import concurrency.concurrent_machine.
+Require Import concurrency.mem_obs_eq.
+Require Import concurrency.dry_context.
+Require Import concurrency.fineConc_safe.
+Require Import Coqlib.
+Require Import msl.Coqlib2.
+
+
+Import dry_context SEM mySchedule DryMachine DryMachine.ThreadPool.
+
+Set Bullet Behavior "None".
+Set Bullet Behavior "Strict Subproofs".
+
+(** ** Safety for X86-SC semantics *)
+Module X86Safe.
+  Import Asm Asm_coop event_semantics FineConcSafe Events.
+
+  Definition sc_init f arg := initial_core x86_sc_semantics the_ge f arg.
+  
+  Notation sc_safe := (X86SC.fsafe the_ge).
+
+  (*TODO: This will be very similar (what an irony) to
+  similar_threadPool, but now we need a more invloved relation on
+  cores that says that things may be more defined. Do we have one? *)
+  
+  Parameter erasePool : FineConc.machine_state -> X86SC.machine_state -> Prop.
+  (** Erasure from FineConc to X86-SC.*)
+  Conjecture x86sc_erasure:
+    forall sched f arg U tpsc tpf m trace
+      (Hmem: init_mem = Some m)
+      (HinitSC: sc_init f arg = Some (U, [::], tpsc))
+      (HinitF: tpf_init f arg = Some (U, [::], tpf))
+      (HsafeF: fsafe tpf m sched trace (size sched).+1),
+      sc_safe tpsc (diluteMem m) sched trace (size sched).+1.
+
+  (** Competing Events *)
+  
+  (* Definition compete (ev1 ev2 : machine_event) (tr : event_trace) : Prop := *)
+  (*   exists n m, *)
+  (*     List.nth_error tr n = Some ev1 /\ *)
+  (*     List.nth_error tr m = Some ev2 /\ *)
+  (*     thread_id ev1 <> thread_id ev2 /\ *)
+      
+End X86Safe.
+
+  
+  
+
+
+
